\documentclass{article}

\input{defs}

\title{Linear Transformations and Matrices - a short Review}
\author{Peleg Bar Sapir}

\begin{document}
\maketitle

\section{Introduction}
\subsection{Transformations on Vectors}
\subsection{Examples of Core LTs in $\Rs[2]$}

\section{Definition and Properties of LTs}

\section{Vectors and Basis Sets}

\section{From LTs to Matrices}

\section{The Determinant}
\subsection{Definition and Properties}
\subsection{Calculating the Determinant}
In $\Rs[2]$ the determinant of two vectors $\vec{a}$ and $\vec{b}$ is simply the area of the parallelogram spanned by the two vectors (\autoref{fig:area_two_vecs}).

\begin{figure}
	\begin{center}
		\begin{tikzpicture}
			\coordinate (a) at (3,1);
			\coordinate (b) at (1,2);
			\fill[xpurple!35] (0,0) -- (a) -- ++(b) -- (b) -- cycle;
			\node[fit={(0,0) (a) ($(a)+(b)$) (b)}] {$A$};
			\draw[vector={xred}]  (0,0) -- (a) node [midway, below right] {$\vec{a}$};
			\draw[vector={xblue}] (0,0) -- (b) node [midway, above left]  {$\vec{b}$};
			\draw[vector={xred}, dashed]  (b) -- ++(a) node [midway, above left]   {$\vec{a}$};
			\draw[vector={xblue}, dashed] (a) -- ++(b) node [midway, below right]  {$\vec{b}$};
		\end{tikzpicture}
	\end{center}
	\caption{The area of the parallelogram spanned by two vectors $\vec{a}$ and $\vec{b}$.}
	\label{fig:area_two_vecs}
\end{figure}

Let's check several properties of this area:
\begin{enumerate}
	\item The parallelogram spanned by the two basis vectors $\eb{1}$ and $\eb{2}$ has an area of $1$: $A\left(\eb{1},\eb{2}\right)=1$.
	\item If the two vectors are on the same line then the area equals $0$, i.e. $A\left(\vec{a}, \lambda\vec{a}\right)=0$, where $\lambda\in\Rs$.
	\item The parallelogram spanned by one vector $\vec{a}$ and a sum of two vectors $\vec{b}+\vec{c}$ has the same area as the sum of the areas of the two parallelograms spanned by $\vec{a},\ \vec{b}$ and by $\vec{a},\ \vec{c}$: $A\left(\vec{a},\vec{b}+\vec{c}\right)=A\left(\vec{a},\vec{b}\right)+A\left(\vec{a},\vec{c}\right)$ (\autoref{fig:adding_parallelograms}).
	\item Scaling any of the two vectors scales the area by the same factor: $A\left(\alpha\vec{a},\beta\vec{b}\right)=\alpha\beta A\left(\vec{a},\vec{b}\right)$, where $\alpha,\beta\in\Rs$ (\autoref{fig:scaling_parallelogram}). A special case of scaling is that of scaling by a negative scalar: for example, $A\left(-\vec{a},\vec{b}\right)=-A\left(\vec{a},\vec{b}\right)$.
\end{enumerate}

\begin{figure}
	\begin{subfigure}[b]{0.3\textwidth}
		\begin{center}
			\begin{tikzpicture}
				\coordinate (a) at (3,1);
				\coordinate (b) at (1,2);
				\coordinate (c) at (-1,2);
				\coordinate (d) at ($(b)+(c)$);
				\draw[vector={xred}]  (0,0) -- (a) node [midway, below right] {$\vec{a}$};
				\draw[vector={xblue}] (0,0) -- (b) node [midway, above left]  {$\vec{b}$};
				\draw[vector={xgreen}] (0,0) -- (c) node [midway, left]  {$\vec{c}$};
				\draw[vector={xorange}] (0,0) -- (d) node [midway, above left]  {$\vec{b}+\vec{c}$};
			\end{tikzpicture}
			\caption{}
		\end{center}
	\end{subfigure}
	\hfill
	\begin{subfigure}[b]{0.3\textwidth}
		\begin{center}
			\begin{tikzpicture}
				\coordinate (a) at (3,1);
				\coordinate (b) at (1,2);
				\coordinate (c) at (-1,2);
				\coordinate (d) at ($(b)+(c)$);
				\fill[xpurple!35] (0,0) -- (a) -- ++(d) -- (d) -- cycle;
				\node[fit={(0,0) (a) ($(a)+(d)$) (d)}] {$A_{1}$};
				\draw[vector={xred}]  (0,0) -- (a) node [midway, below right] {$\vec{a}$};
				\draw[vector={xorange}] (0,0) -- (d) node [midway, above left]  {$\vec{b}+\vec{c}$};
				\draw[vector={xred}, dashed]  (d) -- ++(a);
				\draw[vector={xorange}, dashed] (a) -- ++(d);
			\end{tikzpicture}
			\caption{}
		\end{center}
	\end{subfigure}
	\hfill
	\begin{subfigure}[b]{0.3\textwidth}
		\begin{center}
			\begin{tikzpicture}
				\coordinate (a) at (3,1);
				\coordinate (b) at (1,2);
				\fill[xpurple!35] (0,0) -- (a) -- ++(b) -- (b) -- cycle;
				\node[fit={(0,0) (a) ($(a)+(b)$) (b)}] {$A_{2}$};
				\draw[vector={xred}]  (0,0) -- (a) node [midway, below right] {$\vec{a}$};
				\draw[vector={xblue}] (0,0) -- (b) node [midway, above left]  {$\vec{b}$};
				\draw[vector={xred}, dashed]  (a) -- ++(b);
				\draw[vector={xblue}, dashed] (b) -- ++(a);
			\end{tikzpicture}
			\caption{}
		\end{center}
	\end{subfigure}
	\hfill
	\begin{subfigure}[b]{0.3\textwidth}
		\begin{center}
			\begin{tikzpicture}
				\coordinate (a) at (3,1);
				\coordinate (c) at (-1,2);
				\fill[xpurple!35] (0,0) -- (a) -- ++(c) -- (c) -- cycle;
				\node[fit={(0,0) (a) ($(a)+(c)$) (c)}] {$A_{3}$};
				\draw[vector={xred}]   (0,0) -- (a) node [midway, below right] {$\vec{a}$};
				\draw[vector={xgreen}] (0,0) -- (c) node [midway, left]  {$\vec{c}$};
				\draw[vector={xred}, dashed] (a) -- ++(c);
				\draw[vector={xgreen}, dashed] (c) -- ++(a);
			\end{tikzpicture}
			\caption{}
		\end{center}
	\end{subfigure}
	\hfill
	\begin{subfigure}[b]{0.3\textwidth}
		\begin{center}
			\begin{tikzpicture}
				\coordinate (a) at (3,1);
				\coordinate (b) at (1,2);
				\coordinate (c) at (-1,2);
				\coordinate (d) at ($(b)+(c)$);
				\draw[vector={xred}]    (0,0) -- (a);
				\draw[vector={xblue}]   (0,0) -- (b);
				\draw[vector={xgreen}]  (0,0) -- (c);
				\draw[vector={xorange}] (0,0) -- (d);
				\draw[vector={xred}, dashed] (b) -- ++(a);
				\draw[vector={xred}, dashed] (c) -- ++(a);
				\draw[vector={xred}, dashed] (d) -- ++(a);
				\draw[vector={xblue}, dashed] (a) -- ++(b);
				\draw[vector={xgreen}, dashed] (a) -- ++(c);
				\draw[vector={xorange}, dashed] (a) -- ++(d);
				\draw[vector={xblue}, dashed] (c) -- ++(b);
				\draw[vector={xblue}, dashed] ($(a)+(c)$) -- ++(b);
				\draw[vector={xgreen}, dashed] (b) -- ++(c);
				\draw[vector={xgreen}, dashed] ($(a)+(b)$) -- ++(c);
			\end{tikzpicture}
			\caption{}
		\end{center}
	\end{subfigure}
	\hfill
	\caption{The area of the parallelogram spanned by the vectors $\vec{a}$ and $\vec{b}+\vec{c}$: (a) all four vectors, (b)-(d) the areas of the differenct parallelograms $A_{1}=A\left(\vec{a},\vec{b}+\vec{c}\right),\ A_{2}=A\left(\vec{a},\vec{b}\right),\ A_{3}=A\left(\vec{a},\vec{c}\right)$. In (e) we see that adding the areas $A_{2}$ and $A_{3}$ gives us the area $A_{1}$.}
	\label{fig:adding_parallelograms}
\end{figure}

\begin{figure}
	\begin{center}
		\begin{tikzpicture}
			\coordinate (a) at (3,1);
			\coordinate (b) at (1,2);
			\fill[xpurple!35] (0,0) -- ($2*(a)$) -- ++(b) -- (b) -- cycle;
			\node[fit={(0,0) (a) ($(a)+(b)$) (b)}] {$A$};
			\node[fit={(a) ($2*(a)$) ($2*(a)+(b)$) ($(a)+(b)$)}] {$A$};
			\draw[vector={xred}]  (0,0) -- (a) node [midway, below right] {$\vec{a}$};
			\draw[vector={xblue}] (0,0) -- (b) node [midway, above left]  {$\vec{b}$};
			\draw[vector={xred}, dashed]  (b) -- ++(a) node [midway, above left] {$\vec{a}$};
			\draw[vector={xblue}, dashed] (a) -- ++(b) node [midway, right] {$\vec{b}$};
			\draw[vector={xred}, dashed]  (a) -- ++(a) node [midway, below right] {$\vec{a}$};
			\draw[vector={xblue}, dashed] ($2*(a)$) -- ++(b) node [midway, right] {$\vec{b}$};
			\draw[vector={xred}, dashed]  ($(a)+(b)$) -- ++(a) node [midway, above left] {$\vec{a}$};
		\end{tikzpicture}
	\end{center}
	\caption{Scaling the vector $\vec{a}$ by a factor of $2$ scales the area of the parallelogram by the same factor.}
	\label{fig:scaling_parallelogram}
\end{figure}

Using the above properties, we can derive the relation between $A\left(\vec{a},\vec{b}\right)$ and $A\left(\vec{b},\vec{a}\right)$:
\begin{equation}
	\begin{aligned}
		A\left(\vec{a},\vec{b}\right) & = \cancel{A\left(\vec{a}+\vec{b},\vec{b}+\vec{a}\right)} - A\left(\vec{b},\vec{a}\right) \\
		                              & = -A\left(\vec{b},\vec{a}\right).
	\end{aligned}
	\label{eq:sqapping_order_of_vectors_area_paeallelogram}
\end{equation}
This means that swapping the order of vectors in the area of a parallelogram changes its sign.

Now we can calculate the area of the parallelogram spanned by two vectors $\vec{a}=a_{x}\xhat+a_{y}\yhat$ and $\vec{b}=b_{x}\xhat+b_{y}\yhat$:
\begin{equation}
	\begin{aligned}
		A\left(\vec{a},\vec{b}\right) &= A\left(a_{x}\xhat+a_{y}\yhat, b_{x}\xhat+b_{y}\yhat\right)\\
									  &= A\left(a_{x}\xhat+a_{y}\yhat, b_{x}\xhat\right) + A\left(a_{x}\xhat+a_{y}\yhat, b_{y}\yhat\right)\\
									  &= \cancel{A\left(a_{x}\xhat, b_{x}\xhat\right)} + A\left(a_{y}\yhat, b_{x}\xhat\right) + A\left(a_{x}\xhat, b_{y}\yhat\right) + \cancel{A\left(a_{y}\yhat, b_{y}\yhat\right)}\\
									  &= a_{y}b_{x}A\left(\yhat,\xhat\right) + a_{x}b_{y}A\left(\xhat,\yhat\right)\\
									  &= a_{y}b_{x}(-1) + a_{x}b_{y}(1)\\
									  &= a_{x}b_{y} - a_{y}b_{x}.
	\end{aligned}
	\label{eq:label}
\end{equation}

\subsection{Matrix Rank and Null Space}

\section{Matrix-Matrix Products}

\section{Eigenvalues and Eigenvectors}

\end{document}
